devel/Iron/Language/SystemF2Effect/Type/TyCap.v
@@ -1,0 +1,8 @@
+
+Require Export Iron.Language.SystemF2Effect.Kind.
+
+
+(* Type level capabilities *)
+Inductive tycap : Type :=
+ | TyCapRegion   : nat -> tycap.
+Hint Constructors tycap.
